thys/Substitution/Expressions.thy
@@ -137,6 +137,7 @@ lemma Ector_fresh_inject:
   apply blast
   done
 
+
 end
 
 end
